src/arch/x64/X64.Vale.QuickCodes_i.fsti
@@ -194,7 +194,7 @@ let eval_cmp (s:state) (c:cmp) : GTot bool =
 [@va_qattr]
 let wp_If (#a:Type) (#c1:code) (#c2:code) (b:cmp) (qc1:quickCode a c1) (qc2:quickCode a c2) (s0:state) (k:state -> a -> Type0) : Type0 =
   // REVIEW: this duplicates k
-  valid_cmp b s0 /\ (eval_cmp s0 b ==> QProc?.wp qc1 ({s0 with trace=BranchPredicate(true)::s0.trace}) k) /\ (not (eval_cmp s0 b) ==> QProc?.wp qc2 ({s0 with trace=BranchPredicate(false)::s0.trace}) k)
+  valid_cmp b s0 /\ (eval_cmp s0 b ==> QProc?.wp qc1 s0 k) /\ (not (eval_cmp s0 b) ==> QProc?.wp qc2 s0 k)
 
 val qIf_monotone (#a:Type) (#c1:code) (#c2:code) (b:cmp) (qc1:quickCode a c1) (qc2:quickCode a c2) (s0:state) (k1:state -> a -> Type0) (k2:state -> a -> Type0) : Lemma
   (requires (forall (s:state) (g:a). k1 s g ==> k2 s g))
@@ -279,13 +279,12 @@ let va_state_match (s0:state) (s1:state) : Pure Type0
   all_xmms_match s0.xmms s1.xmms /\
   s0.flags == s1.flags /\
   s0.mem == s1.mem /\
-  s0.trace == s1.trace /\
   s0.memTaint == s1.memTaint
 
 [@va_qattr]
 unfold let wp_sound_pre (#a:Type0) (#cs:codes) (qcs:quickCodes a cs) (s0:state) (k:state -> state -> a -> Type0) : Type0 =
-  forall (ok:bool) (regs:Regs_i.t) (xmms:Xmms_i.t) (flags:nat64) (mem:mem) (trace:list observation) (memTaint:memtaint).
-    let s0' = {ok = ok; regs = regs; xmms = xmms; flags = flags; mem = mem; trace=trace; memTaint=memTaint} in
+  forall (ok:bool) (regs:Regs_i.t) (xmms:Xmms_i.t) (flags:nat64) (mem:mem) (memTaint:memtaint).
+    let s0' = {ok = ok; regs = regs; xmms = xmms; flags = flags; mem = mem; memTaint=memTaint} in
     s0 == s0' ==> wp cs qcs (k s0') s0'
 
 unfold let wp_sound_post (#a:Type0) (#cs:codes) (qcs:quickCodes a cs) (s0:state) (k:state -> state -> a -> Type0) ((sN:state), (fN:fuel), (gN:a)) : Type0 =
@@ -299,8 +298,8 @@ val wp_sound_wrap (#a:Type0) (cs:codes) (qcs:quickCodes a cs) (s0:state) (k:stat
 
 [@va_qattr]
 unfold let wp_sound_code_pre (#a:Type0) (#c:code) (qc:quickCode a c) (s0:state) (k:state -> state -> a -> Type0) : Type0 =
-  forall (ok:bool) (regs:Regs_i.t) (xmms:Xmms_i.t) (flags:nat64) (mem:mem) (trace:list observation) (memTaint:memtaint).
-    let s0' = {ok = ok; regs = regs; xmms = xmms; flags = flags; mem = mem; trace=trace; memTaint=memTaint} in
+  forall (ok:bool) (regs:Regs_i.t) (xmms:Xmms_i.t) (flags:nat64) (mem:mem) (memTaint:memtaint).
+    let s0' = {ok = ok; regs = regs; xmms = xmms; flags = flags; mem = mem; memTaint=memTaint} in
     s0 == s0' ==> QProc?.wp qc s0' (k s0')
 
 unfold let wp_sound_code_post (#a:Type0) (#c:code) (qc:quickCode a c) (s0:state) (k:state -> state -> a -> Type0) ((sN:state), (fN:fuel), (gN:a)) : Type0 =
@@ -318,21 +317,21 @@ val wp_sound_code_wrap (#a:Type0) (c:code) (qc:quickCode a c) (s0:state) (k:stat
 [@va_qattr]
 let wp_final_k (#a:Type0) (update:state -> state) (post:state -> state -> Type0) (k:state -> a -> Type0) (sN:state) (g:a) : Type0 =
   va_state_match sN (update sN) /\ post sN sN /\
-    (forall (ok':bool) (regs':Regs_i.t) (xmms':Xmms_i.t) (flags':nat64) (mem':mem) (trace':list observation) (memTaint':memtaint).
-      let sN' = {ok = ok'; regs = regs'; xmms = xmms'; flags = flags'; mem = mem'; trace=trace'; memTaint=memTaint'} in
+    (forall (ok':bool) (regs':Regs_i.t) (xmms':Xmms_i.t) (flags':nat64) (mem':mem) (memTaint':memtaint).
+      let sN' = {ok = ok'; regs = regs'; xmms = xmms'; flags = flags'; mem = mem'; memTaint=memTaint'} in
       post sN sN' ==> k sN' g)
 
 // For efficiency, introduce shorter names (e.g. ok, mem) for components of initial state s0.
 [@va_qattr]
 let wp_wrap (#a:Type0) (cs:codes) (qcs:quickCodes a cs) (update:state -> state -> state) (post:state -> state -> Type0) (k:state -> a -> Type0) (s0:state) : Type0 =
-  forall (ok:bool) (regs:Regs_i.t) (xmms:Xmms_i.t) (flags:nat64) (mem:mem) (trace:list observation) (memTaint:memtaint).
-    let s0' = {ok = ok; regs = regs; xmms = xmms; flags = flags; mem = mem; trace=trace; memTaint=memTaint} in
+  forall (ok:bool) (regs:Regs_i.t) (xmms:Xmms_i.t) (flags:nat64) (mem:mem) (memTaint:memtaint).
+    let s0' = {ok = ok; regs = regs; xmms = xmms; flags = flags; mem = mem; memTaint=memTaint} in
     s0 == s0' ==> wp cs qcs (wp_final_k (update s0') post k) s0'
 
 [@va_qattr]
 let wp_wrap_code (#a:Type0) (c:code) (qc:quickCode a c) (update:state -> state -> state) (post:state -> state -> Type0) (k:state -> a -> Type0) (s0:state) : Type0 =
-  forall (ok:bool) (regs:Regs_i.t) (xmms:Xmms_i.t) (flags:nat64) (mem:mem) (trace:list observation) (memTaint:memtaint).
-    let s0' = {ok = ok; regs = regs; xmms = xmms; flags = flags; mem = mem; trace=trace; memTaint=memTaint} in
+  forall (ok:bool) (regs:Regs_i.t) (xmms:Xmms_i.t) (flags:nat64) (mem:mem) (memTaint:memtaint).
+    let s0' = {ok = ok; regs = regs; xmms = xmms; flags = flags; mem = mem; memTaint=memTaint} in
     s0 == s0' ==> QProc?.wp qc s0' (wp_final_k (update s0') post k)
 
 unfold let wp_GHOST (#a:Type0) (c:code) (s0:state) (update:state -> state -> state) (fk:(state -> a -> Type0) -> Type0) (p:state * fuel * a -> Type0) : Type0 =
