src/arch/x64/interop/Inc32_win.fst
@@ -38,7 +38,7 @@ B.length stack_b == 16 /\ live h0 stack_b /\ buf_disjoint_from stack_b [iv_b] /\
     | Rcx -> addr_iv_b
     | _ -> init_regs r end in
   let xmms = init_xmms in
-  let s0 = {ok = true; regs = regs; xmms = xmms; flags = 0; mem = mem; trace = []; memTaint = create_valid_memtaint mem buffers taint_func} in
+  let s0 = {ok = true; regs = regs; xmms = xmms; flags = 0; mem = mem; memTaint = create_valid_memtaint mem buffers taint_func} in
   length_t_eq (TBase TUInt64) stack_b;
   length_t_eq (TBase TUInt128) iv_b;
   va_pre (va_code_inc32_buffer_win ()) s0 stack_b iv_b ))) =
@@ -77,7 +77,7 @@ let ghost_inc32_buffer_win iv_b stack_b h0 =
     | Rcx -> addr_iv_b
     | _ -> init_regs r end in
   let xmms = init_xmms in
-  let s0 = {ok = true; regs = regs; xmms = xmms; flags = 0; mem = mem; trace = []; memTaint = create_valid_memtaint mem buffers taint_func} in
+  let s0 = {ok = true; regs = regs; xmms = xmms; flags = 0; mem = mem; memTaint = create_valid_memtaint mem buffers taint_func} in
   length_t_eq (TBase TUInt64) stack_b;
   length_t_eq (TBase TUInt128) iv_b;
   implies_pre h0 iv_b stack_b ;
